partially working!

src/tidy/rewrite_all_2.lean
@@ -7,6 +7,13 @@ universes u
 open tactic
 open mllist
 
+meta def kabstract_no_new_goals (t e : expr) (md : transparency) : tactic expr :=
+do gs ← get_goals,
+   r ← kabstract t e md,
+   ng ← num_goals,
+   guard (ng = gs.length),
+   return r
+
 meta def kabstracter'
   (pattern : tactic (expr × expr × list expr))
   (lhs_replacer : list expr → tactic expr) :
@@ -14,48 +21,48 @@ meta def kabstracter'
 | p := do
   (t, L) ← pure p,
   (e, e_type, mvars) ← pattern,
-  t' ← kabstract t e semireducible,
+  t' ← kabstract_no_new_goals t e semireducible,
+  -- TODO use the discharger to clear remaining metavariables
   -- trace "kabstract:",
+  -- trace t,
+  -- trace e,
+  -- trace mvars,
+  -- mvars.mmap (λ m, infer_type m) >>= trace,
   -- trace t',
   guard t'.has_var,
   w ← mk_meta_var e_type,
   let t'' := t'.instantiate_var w,
   mvars' ← mvars.mmap instantiate_mvars,
-  return (t'', (w, mvars) :: L)
+  return (t'', (w, mvars') :: L) -- FIXME should there be a prime here??
 
 meta def kabstracter 
   (pattern : tactic (expr × expr × list expr))
   (lhs_replacer : list expr → tactic expr) (t : expr) : tactic (mllist tactic (expr × list (expr × list expr))) :=
 mllist.fix (kabstracter' pattern lhs_replacer) (t, [])
 
-meta def substitutions_core : expr → list expr → 
-  tactic (tactic (expr × expr × list expr) × (list expr → tactic expr) × (list expr → tactic expr))
-| (expr.pi n bi d b) types := 
-  do substitutions_core b (d :: types)          
-| `(%%lhs = %%rhs) types := 
-  do let fresh_mvars := (do mvars ← types.mmap mk_meta_var,
-                           let pattern := lhs.instantiate_vars mvars,
-                           ty ← infer_type pattern,
-                           return (pattern, ty, mvars)),
-     let lhs_replacer : list expr → tactic expr := (λ values, return (lhs.instantiate_vars values)),
-     let rhs_replacer : list expr → tactic expr := (λ values, return (rhs.instantiate_vars values)),
-     return (fresh_mvars, lhs_replacer, rhs_replacer)
-| _ _ := failed
+meta def get_lhs : expr -> bool → list expr -> tactic (expr × expr × list expr)
+| (expr.pi n bi d b) symm mvars :=
+do v <- mk_meta_var d,
+   b' <- whnf $ b.instantiate_var v,
+   get_lhs b' symm (v :: mvars)
+| `(%%a = %%b) symm mvars := 
+  do let (a, b) := if symm then (b, a) else (a, b),
+     ty ← infer_type a,
+     return (a, ty, mvars)
+| _ _ _ := failed
 
-/-- Given a lemma `eq`, returns three tactics.
-    1) returning `(lhs, ty, mvars)` where `lhs` is a copy of the left hand side of the lemma, with
-    variables replaced by fresh metavariables `mvars`.
-    2) taking a list of expressions, and returning `lhs'`, the left hand side with variables
-    instantiated with these values.
-    3) as with 2), but for the right hand side. -/
-meta def substitutions (eq : expr) : tactic (tactic (expr × expr × list expr) × (list expr → tactic expr) × (list expr → tactic expr)) :=
-substitutions_core eq []
+meta def replacer : expr -> bool → list expr -> tactic expr
+| (expr.pi n bi d b) symm values := replacer b symm values
+| `(%%a = %%b) symm values := 
+  do let (a, b) := if symm then (b, a) else (a, b),
+     return (a.instantiate_vars values)
+| _ _ _ := failed
 
 meta def mvars_to_var (e : expr) : expr :=
 e.replace (λ e n, if e.is_meta_var then some (expr.var n) else none)
 
 meta def do_substitutions
-  (eq : expr)
+  (eq : expr) (symm : bool)
   (t_original : expr)
   (lhs rhs : list expr → tactic expr)
   (t_abstracted : expr)
@@ -63,11 +70,14 @@ meta def do_substitutions
   (restore_mvars : list (expr × list expr)) : tactic (expr × tactic expr × list expr) :=
 lock_tactic_state $
 do -- We first restore all the "other" metavariables to their original values.
+  --  trace "do_substitutions",
    restore_mvars.mmap (λ p, do l ← lhs p.2, unify p.1 l),
    t_restored ← instantiate_mvars t_abstracted,
 
    -- r' is the value of the remaining metavariable, after applying the lemma.
    r' ← rhs rewrite_mvar.2,
+
+   guard (¬ r'.has_meta_var),
 
    -- We now begin constructing the `eq.rec` proof of equality. In fact, we don't construct it here,
    -- we just construct a tactic that can produce it on demand!
@@ -77,38 +87,57 @@ do -- We first restore all the "other" metavariables to their original values.
 
     -- The lemma itself proves `r = r'`.
     let inner_proof := rewrite_mvar.2.reverse.foldl (λ f x : expr, f x) eq,
+    inner_proof ← if symm then mk_eq_symm inner_proof else return inner_proof,
+    -- trace "inner_proof:",
+    -- trace inner_proof,
 
     -- Next we compute the motive.
     let t_with_var := mvars_to_var t_restored,
     n ← mk_fresh_name,
-    eq ← to_expr ``(%%t_with_var = %%t_original),
+    -- trace "--",
+    -- trace t_with_var,
+    -- trace t_original,
+    -- trace "r:",
+    -- trace r,
     ty ← infer_type r,
-    let C := expr.lam n binder_info.default ty eq,
+    feq ← mk_const `eq,
+    v ← mk_mvar,
+    let C := expr.lam n binder_info.default ty (feq v t_original t_with_var),
+    -- trace "motive:",
+    -- trace C,
 
     -- ... and prepare the actual proof.
     refl ← mk_eq_refl t_original,
     proof ← to_expr ```(@eq.rec _ %%r %%C %%refl _ %%inner_proof),
-    infer_type proof,
+    -- trace "proof:",
+    -- trace proof,
+    infer_type proof, -- this is a sanity check (perhaps we should be doing this earlier?)
     return proof
    },
    -- Finally we finish rewriting the expression
    unify rewrite_mvar.1 r',
    result ← instantiate_mvars t_restored,
 
-   metas : list expr ← rewrite_mvar.2.mfilter (λ m, do r ← is_assigned m, return ¬ r), -- FIXME check if there are any remaining metavariables
+   metas : list expr ← rewrite_mvar.2.mfilter (λ m, do r ← is_assigned m <|> return tt, return ¬ r),
    return (result, proof_tactic, metas)
 
-meta def all_rewrites_core (t eq : expr) : tactic (mllist tactic (expr × tactic expr × list expr)) :=
+meta def all_rewrites_core (t eq : expr) (symm : bool): tactic (mllist tactic (expr × tactic expr × list expr)) :=
 do ty ← infer_type eq,
-  (matcher, lhs, rhs) ← substitutions ty,
+  let matcher := get_lhs ty symm [],
+  let lhs := replacer ty symm,
+  let rhs := replacer ty ¬ symm,
   L ← kabstracter matcher lhs t,
-  L ← L.mmap (λ p, do_substitutions eq t lhs rhs p.1 p.2.head p.2.tail),
+  L ← L.mmap (λ p, do_substitutions eq symm t lhs rhs p.1 p.2.head p.2.tail),
   return L
 
-meta def all_rewrites' (t eq : expr) : tactic (list (expr × expr × list expr)) :=
-do L ← all_rewrites_core t eq,
+meta def all_rewrites' (t eq : expr) (symm : bool) : tactic (list (expr × expr × list expr)) :=
+do L ← all_rewrites_core t eq symm,
    L' ← L.mmap (λ p, do r ← p.2.1, return (p.1, r, p.2.2)),
-   L'.force
+   R ← L'.force,
+  --  trace "all_rewrite':",
+  --  trace (t, eq, symm),
+  --  trace R,
+   return R
   
 constant f (x : ℕ) (y : ℕ) : ℕ
 axiom fx (n : ℕ) (m : ℕ) : f n m = f 17 19
@@ -117,7 +146,7 @@ example : [f 1 2, 3, f 2 5] = [f 1 2, 3, f 2 5] :=
 begin
 (do `(%%lhs = %%rhs) ← target,
     eq ← mk_const `fx,
-    r ← all_rewrites' lhs eq,
+    r ← all_rewrites' lhs eq ff,
     trace r),
 refl
 end
@@ -127,9 +156,7 @@ meta structure rewrite_all_cfg extends rewrite_cfg :=
 (simplifier : expr → tactic (expr × expr) := λ e, failed) -- FIXME get rid of this
 
 meta def all_rewrites (r : expr × bool) (t : expr) (cfg : rewrite_all_cfg := {}): tactic (list (expr × expr)) :=
-do e ← if r.2 then mk_eq_symm r.1 else return r.1,
-   results ← all_rewrites' t e,
-   -- TODO use the discharger to clear remaining metavariables
+do results ← all_rewrites' t r.1 r.2,
    let results := results.filter (λ p, p.2.2 = []),
    let results := results.map (λ p, (p.1, p.2.1)),
    return results
